tutorial/lithium/primitive_laws.v
@@ -18,10 +18,10 @@ Global Instance tutorial_irisG `{!tutorialGS Σ} : irisGS tutorial_lang Σ := {
   state_interp_mono _ _ _ _ := fupd_intro _ _;
 }.
 
-Definition val_mapsto `{!tutorialGS Σ} (v1 : val) (dq : dfrac) (v2 : val) : iProp Σ :=
-  ∃ l : loc, ⌜v1 = #l⌝ ∗ mapsto l dq v2.
+Definition val_pointsto `{!tutorialGS Σ} (v1 : val) (dq : dfrac) (v2 : val) : iProp Σ :=
+  ∃ l : loc, ⌜v1 = #l⌝ ∗ pointsto l dq v2.
 
-Notation "v1 ↦ dq v2" := (val_mapsto v1 dq v2)
+Notation "v1 ↦ dq v2" := (val_pointsto v1 dq v2)
   (at level 20, dq custom dfrac at level 1, format "v1  ↦ dq  v2") : bi_scope.
 
 
@@ -32,9 +32,9 @@ Section lifting.
   Lemma wp_alloc s E Φ :
     (∀ v, v ↦ #0 -∗ Φ v) -∗ WP Alloc @ s; E {{ Φ }}.
   Proof.
-    iIntros "HΦ". iApply wp_lift_atomic_head_step_no_fork; first done.
-    iIntros (σ1 κ κs n nt) "Hσ !>"; iSplit; first by auto with head_step.
-    iIntros "!>" (v2 σ2 efs Hstep) "_Hcred"; inv_head_step.
+    iIntros "HΦ". iApply wp_lift_atomic_base_step_no_fork; first done.
+    iIntros (σ1 κ κs n nt) "Hσ !>"; iSplit; first by auto with base_step.
+    iIntros "!>" (v2 σ2 efs Hstep) "_Hcred"; inv_base_step.
     iMod (gen_heap_alloc with "Hσ") as "[Hσ [Hl _]]"; first done.
     iModIntro; iSplit=> //. iFrame. iApply "HΦ". iExists _. by iFrame.
   Qed.
@@ -42,25 +42,25 @@ Section lifting.
   Lemma wp_load s E Φ v1 v2 :
     v1 ↦ v2 -∗ (v1 ↦ v2 -∗ Φ v2) -∗ WP Load v1 @ s; E {{ Φ }}.
   Proof.
-    iIntros "[%l [-> Hl]] HΦ". iApply wp_lift_atomic_head_step_no_fork; first done.
+    iIntros "[%l [-> Hl]] HΦ". iApply wp_lift_atomic_base_step_no_fork; first done.
     iIntros (σ1 κ κs n nt) "Hσ !>".
     iDestruct (gen_heap_valid with "Hσ Hl") as %?.
-    iSplit; first by eauto with head_step.
-    iIntros "!>" (? σ2 efs Hstep) "_Hcred"; inv_head_step.
+    iSplit; first by eauto with base_step.
+    iIntros "!>" (? σ2 efs Hstep) "_Hcred"; inv_base_step.
     iModIntro; iSplit=> //. iFrame. iApply "HΦ". iExists _. by iFrame.
   Qed.
 
   Lemma wp_store s E Φ v1 v (w : val) :
     v1 ↦ v -∗ (v1 ↦ w -∗ Φ w) -∗ WP Store v1 w @ s; E {{ Φ }}.
   Proof.
-    iIntros "[%l [-> Hl]] HΦ". iApply wp_lift_atomic_head_step_no_fork; first done.
+    iIntros "[%l [-> Hl]] HΦ". iApply wp_lift_atomic_base_step_no_fork; first done.
     iIntros (σ1 κ κs n nt) "Hσ !>".
     iDestruct (gen_heap_valid with "Hσ Hl") as %?.
-    iSplit; first by eauto with head_step.
-    iIntros "!>" (v2 σ2 efs Hstep) "_Hcred"; inv_head_step.
+    iSplit; first by eauto with base_step.
+    iIntros "!>" (v2 σ2 efs Hstep) "_Hcred"; inv_base_step.
     iMod (gen_heap_update with "Hσ Hl") as "[Hσ Hl]".
     iModIntro; iSplit=> //. iFrame. iApply "HΦ". iExists _. by iFrame.
   Qed.
 End lifting.
 
-Global Typeclasses Opaque val_mapsto.
+Global Typeclasses Opaque val_pointsto.
